<font face="Times New Roman">

# Discrete Mathematics Homework 2

## Section 2-4

**8 . Find at least three different sequences beginning with the terms 3, 5, 7 whose terms are generated by a simple formula or rule.**
1. $\{a_n\}:a_n=2n+1, n\in{\mathbb{N}}$
2. $\{a_n\}:a_n=2^n+3, n\in{\mathbb{N}}$
3. $\{a_n\}:a_n=a_{n-1}+a_{n-2}-1, a_1=3, a_2=5, n=3,4,5...$

**14 . For  each  of  these  sequences  find  a  recurrence  relation satisfied by this sequence. ( The answers are not unique because  there  are  infinitely  many  different  recurrence relations satisfied by any sequence.)**
- (b) $a_n=2n$
  - $a_n=a_{n-1}+2$
- (h) $a_n=n!$
  - $a_n=na_{n-1}$

**16 . Find the solution to each of these recurrence relations with the given initial conditions. Use an iterative approach such as that used in Example 10.**
- (d) $a_n=2a_{n-1}-3, a_0=-1$
  - $a_n=2a_{n-1}-3$
    $=2(2a_{n-2}-3)-3=2^2a_{n-2}-3\times{(1+2)}$
    $=4(2a_{n-3}-3)-9=2^3a_{n-3}-3\times{(1+2+3)}$
    $=2^ia_{n-i}-3\times{\frac{1(2^i-1)}{2-1}}$
    $=2^na_0-3\times{(2^n-1)}$
    $=-2^n-3\times{2^n}+3$
    $=3-2^{n+2}$

**34 . Compute each of these double sums.**
- (d) $\sum\limits_{i=0}^{2}\sum\limits_{j=0}^{3}i^2j^3$
  $=\sum\limits_{i=0}^{2}(i^2(\frac{3^2\times{4^2}}{4}))=\sum\limits_{i=0}^236i^2=36\times{\frac{2\times{3}\times{5}}{6}}=180$

## Section 4-1

**14 . Suppose that $a$ and $b$ are integers, $a\equiv{11}(mod$ $19)$ and $b\equiv{3}(mod$ $19)$. Find the integer $c$ with $0\leq{c}\leq{18}$ such that**
- (d) $c\equiv 7a+3b$ $(mod$ $19).$
  - $c\equiv 7a+3b\equiv 7\times{11}+3\times{3}\equiv{86}\equiv{10}.$

**34 . Show that if $a\equiv{b}$ $(mod$ $m)$ and $c\equiv{d}$ $(mod$ $m)$, where $a,b,c,d$ and $m$ are integers with $m\geq{2}$, then $a-c\equiv{b}-d$ $(mod$ $m)$.**
- ***There are integers $s,t$ with $a=b+ms,c=d+mt$, then***
  $a-c=(b+ms)-(d+mt)=(b-d)+m(s-t)$
  ***So $a-c\equiv{b}-d$ $(mod$ $m)$.***

**38 . Show that if $n$ is an integer then $n^2\equiv{0}$ or $1 (mod$ $4)$.**
1. ***$n$ is even: $n=2k, k\in{\mathbb{N}^0} \Rightarrow n^2=4k^2\equiv{0}$ $(mod$ $4).$***
2. ***$n$ is odd: $n=2k+1, k\in{\mathbb{N}^0}\Rightarrow n^2=(2k+1)^2=4(k^2+k)+1\equiv{1}$ $(mod$ $4).$***

## Section 4-2

**2 . Convert the decimal expansion of each of these integers to a binary expansion.**
- (c) $100632=(11000100100011000)_{2}$

**4 . Convert the binary expansion of each of these integers to a decimal expansion.**
- (c) $(11 1011 1110)_{2}=958$

**8 . Convert $(BADFACED)_{16}$ from its hexadecimal expansion to its binary expansion.**
- $(10111010110111111010110011101101)_{2}$

**22 . Find the sum and product of each of these pairs of numbers. Express your answers as a base $3$ expansion.**
- (b) $(2112)_{3},(12021)_{3}$
  - ***Sum : $(21210)_{3}$***
  - ***Product : $(111020122)_{3}$***

**28 . Use Algorithm $5$ to find $123^{1001} mod$ $101$.**
- $87$

## Section 4-3

**10 . Show that if $2^m+1$ is an odd prime , then $m=2^n$ for some nonnegative interger $n$. [Hint : First show that the ploynomial identity $x^m+1=(x^k+1)(x^{k(t-1)}-x^{k(t-2)}+...-x^k+1)$ holds, where $m=kt$ and $t$ is odd.]**
- ***We want to show that if $m\neq{2^n}$, then $2^m+1$ is not an odd prime. Let $t$ be an odd prime so that $m=kt$, where $k=\frac{m}{t}$ is a positive integer, then $2^m+1=(2^k+1)(2^{k(t-1)}-...)$. To have $2^m+1$ an odd prime, we must have $m=k$ and $t=1$, which is cotradict to "$t$ is an odd prime", so $2^m+1$ can't be an odd prime if $m$ can not only be divided by 2.***

**12 . Prove that for every positive integer $n$, there are $n$ consecutive composite integers. [Hint : Consider the $n$ consecutive integers strating with $(n+1)!+2.$]**
- $2|(n+1)!+2,\ 3|(n+1)!+3,\ ......, n|(n+1)!+n,\ n+1|(n+1)!+(n+1)$
  ***So there are $n$ consecutive composite integers since $k|(n+1)!+k,\ \forall 2\leq{k}\leq{n+1}$***

**16 . Determine whether the integers in each of these sets are pairwise relatively prime.**
- (c) $25,41,49,64$
  - ***These numbers are whether perfect squares or primes, so they are pairwise relatively prime.***

**28 . Find $gcd(1000,625)$ and $lcm(1000,625)$ and verify that $gcd(1000,625)\cdot lcm(1000,625)=1000\cdot{625}$**
- $gcd(1000,625)=125$
- $lcm(1000,625)=5000$
- $gcd(1000,625)\cdot lcm(1000,625)=125\cdot{5000}=1000\cdot{625}$

**32 . Use the Euclidean algorithm to find**
- (c) $gcd(123,277)=1$

**52 . Prove or disprove that $p_1p_2...p_n+1$ is prime for every positive integer $n$, where $p_1,p_2,...,p_n$ are the $n$ smallest prime numbers.**
- ***It doesn't hold at $n=6 (2\times 3\times 5\times 7\times 11\times 13 +1 = 30031 = 59\times{509})$.***

# Section 4-4

**6 . Find an inverse of $a$ modulo $m$ for each of these pairs of relatively prime integers using the method followed in Example 2.**
- (a) $a=2,m=17$
  - $17=8\times{2}+1$
    $\Rightarrow -8\times{2}+17=1$
    $\Rightarrow -8\times{2}\equiv{1}$ $(mod$ $17)$
    $\bar{a}=-8$
- (c) $a=144,m=233$
  - |Euclidean||Bezout|
    |--|--|:--|
    |$233=144+89$|\||$1=3-2=3-(5-3)=-5+(2\times{3})$|
    |$144=89+55$|\||$=-5+2\times{(8-5)}=2\times{8}-3\times{5}$|
    |$89=55+34$|\||$=2\times{8}-3\times{(13-8)}=-3\times{13}+5\times{8}$|
    |$55=34+21$|\||$=-3\times{13}+5\times{(21-13)}=5\times{21}-8\times{13}$|
    |$34=21+13$|\||$=5\times{21}-8\times{(34-21)}=-8\times{34}+13\times{21}$|
    |$21=13+8$|\||$=-8\times{34}+13\times{(55-34)}=13\times{55}-21\times{34}$|
    |$13=8+5$|\||$=13\times{55}-21\times{(89-55)}=-21\times{89}+34\times{55}$|
    |$8=5+3$|\||$=-21\times{89}+34\times{(144-89)}=34\times{144}-55\times{89}$|
    |$5=3+2$|\||$=34\times{144}-55\times{(233-144)}=-55\times{233}+89\times{144}$|
    |$3=2+1$|\|||
    So $\bar{a}=89.$

**12 . Solve each of these congruences using the modular inverses found in parts (b), (c), and (d) of Exercise 6.**
- (b) $144x\equiv 4$ $(mod$ $233)$
  - $4\times{89}=356\equiv{123}$ $(mod$ $233)$
    $x=233$

**20 . Use the construction in the proof of the Chinese remainder theorem to find all solutions to the system of congruence $x\equiv 2$ $(mod$ $3)$, $x\equiv 1$ $(mod$ $4)$, and $x\equiv 3$ $(mod$ $5)$**
- $m_1=3, m_2=4, m_3=5, m=3\times 4\times 5=60$
  $M_1=20, M_2=15, M_3=12, y_1=2, y_2=3, y_3=3$
  $x= 2\times{20}\times{2}+1\times{15}\times{3}+3\times{12}\times{3}=233\equiv{53}$ $(mod$ $60)$
  $\forall{x}\in{\{x|53+60n, \forall{n}\in{\mathbb{Z}^+}\}}$

**38 . Use Fermat’s little theorem to compute $3^{302} mod$ $5$, $3^{302} mod$ $7$, and $3^{302} mod$ $11$. Then use your results above and the Chinese remainder theorem to find $3^{302} mod$ $385$ $(385=5\times 7\times 11)$.**
- $3^{302}$ $mod$ $5 :$
  - $3^4\equiv{1}\ (mod\ 5)$
    $3^{300}\equiv 1\ (mod \ 5)$
    $3^{300}\times 3^2\equiv 3^2\ (mod \ 5)$
    $3^2\equiv 4\ (mod \ 5)$
    $3^{302}\equiv 4\ (mod \ 5)$
- $3^{302}$ $mod$ $7 :$
  - $3^6\equiv1\ (mod \ 7)$
    $3^{302}\equiv 3^2\equiv 2\ (mod\ 7)$
- $3^{302}$ $mod$ $11 :$
  - $3^{10}\equiv 1\ (mod\ 11)$
    $3^{302}\equiv 3^2\equiv 9\ (mod\ 11)$

**40 . Show with the help of Fermat’s little theorem that if $n$ is a positive integer, then $42$ divides $n^7-n$.**
- $42=2\times 3\times 7$
- $2|n^7-n:$ ***$n^7-n$ will be even either $n$ is odd or even.***
- $3|n^7-n:n^7-n\equiv{(n^2)^3\times{n}-n}\equiv 1\times{n}-n\equiv{0}\ (mod\ 3).$
- $7|n^7-n:n^7-n\equiv n^6\times{n}-n\equiv 1\times{n}-n\equiv{0}\ (mod\ 7).$

## Section 4-6

**24 . Encrypt the message ATTACK using the RSA system with $n=43\times{59}$ and $e=13$, translating each letter into integers and grouping together pairs of integers, as done in Example 8.**
- $e=13,n=43\times 59=2537$
  $AT=0019,TA=1900,CK=0210$
  $19^{13}\equiv2299\ (mod\ 2537)$
  $1900^{13}\equiv1317\ (mod\ 2537)$
  $210^{13}\equiv2117\ (mod\ 2537)$
  ***So ATTACK means :*** $2299\ 1317\ 2117$

**26 . What is the original message encrypted using the RSA system with $n=53\times 61$ and $e=17$ if the encrypted message is $3185 2038 2460 2550$? (To decrypt, first find the decryption exponent $d$, which is the inverse of $e=17$ modulo $52\times{60}$.)**
- $d=e^{-1}=2753\ (mod\ 52*60)$
  $n=53*61=3233$
  $3185^{2753}\equiv1816\ (mod\ 3233)\to SQ$
  $2038^{2753}\equiv2008\ (mod\ 3233)\to UI$
  $2460^{2753}\equiv1717\ (mod\ 3233)\to RR$
  $2550^{2753}\equiv0411\ (mod\ 3233)\to EL$
  ***So $3185\ 2038\ 2460\ 2550$ means : SQUIRREL***

## Section 5-1

**8 . Prove that $2-2\times 7+2\times7^2 -...+2(-7)^n =\frac{(1- (-7)^{n+1})}{4}$ whenever $n$ is a nonnegative integer.**
- $Basis\ Step : n=0,\frac{1- (-7)}{4}=2$
- $Inductive\ Step :$ ***assume that when*** $n=k, \sum\limits_{i=0}^{k}2(-7)^i=\frac{(1- (-7)^{k+1})}{4}$
  ***Then when*** $n=k+1, \sum\limits_{i=0}^{k+1}2(-7)^i=\frac{(1- (-7)^{k+1})}{4}+2(-7)^{k+1}=\frac{1- (-7)^{k+1}+8(-7)^{k+1}}{4}=\frac{1-(-7)^{k+2}}{4}$
  ***So $\forall{n\in\mathbb{Z}^+}(\sum\limits_{i=0}^{n}2(-7)^i=\frac{(1-(-7)^{n+1})}{4})$***

**32 . Prove that $3$ divides $n^3+2n$ whenever $n$ is a positive integer.**
- $Basis\ Step : n=0, n^3+2n=3$
- $Inductive\ Step :$ ***assume that when*** $n=k, 3|k^3+2k$
  ***Then when*** $n=k+1, (k+1)^3+2(k+1)=k^3+3k^2+3k+1+2k+2=(k^3+2k)+3(k^2+k+1)\equiv{0}\ (mod\ 3)$

**38 . Prove that if $A_1,A_2,...,A_n$ and $B_1,B_2,...,B_n$ are sets such that $A_j\subseteq B_j$ for $j = 1,2,...,n$, then$\bigcup\limits_{j=1}^{n}A_j\subseteq\bigcup\limits_{j=1}^{n}B_j$**
- $Basis\ Step : \bigcup\limits_{j=1}^{1}A_j=A_1\subseteq \bigcup\limits_{j=1}^{1}B_j=B_1$
- $Inductive\ Step :$ ***assume that when*** $n = k,$ $\forall{j\in\{1,2,...,k\}((A_j\subseteq B_j)\to(\bigcup\limits_{j=1}^{k}A_j\subseteq\bigcup\limits_{j=1}^{k}B_j))}$
  ***Then when*** $n=k+1:$  
  ***Let $x\in\bigcup\limits_{j=1}^{k+1}A_j=(\bigcup\limits_{j=1}^{k}A_j)\cup A_{k+1}.$ From the hypothesis we know that $x\in\bigcup\limits_{j=1}^{k}A_j\to x\in\bigcup\limits_{j=1}^{k}B_j$, and form the given fact we know that $A_{k+1}\subseteq B_{k+1}$, that is, $x\in A_{k+1}\to x\in B_{k+1}$. Therefore, in either case $x\in(\bigcup\limits_{j=1}^{k}B_j)\cup B_{k+1}$***

**56 . Suppose that $A=\begin{bmatrix}a&0\\0&b\end{bmatrix}$, where $a$ and $b$ are real numbers. Show that $A^n=\begin{bmatrix}a^n&0\\0&b^n\end{bmatrix}$ for every positive interger $n$.**
- $Basis\ Step : A=A$
- $Inductive\ Step :$ ***assume that when*** $n = k, A^k=\begin{bmatrix}a^k&0\\0&b^k\end{bmatrix}$  
  ***Then when*** $n=k+1: A^{k+1}=AA^k=\begin{bmatrix}a&0\\0&b\end{bmatrix}\begin{bmatrix}a^k&0\\0&b^k\end{bmatrix}=\begin{bmatrix}a^{k+1}&0\\0&b^{k+1}\end{bmatrix}$
  ***Thus*** $\forall{n\in{\mathbb{N}}}(A^n=\begin{bmatrix}a^n&0\\0&b^n\end{bmatrix})$

## Section 5-2

**6 . ...**
- (a) Determine which amounts of postage can be formed using just $3$-cent and $10$-cent stamps.
  - |denomination|combination|denomination|combination|
    |--|--|--|--|
    |3|3|15|3+3+3+3+3|
    |6|3+3|16|10+3+3|
    |9|3+3+3|18|3+3+3+3+3+3|
    |10|10|19|10+3+3+3|
    |12|3+3+3+3|20|10+10|
    |13|10+3|...||
    ***Claim: We can form any amount of postages greater than or equal to 18 cents using just 3-cent stamps and 10-cent stamps.***
- (b) Prove your answer to (a) using the principle of mathematical induction. Be sure to state explicitly your inductive hypothesis in the inductive step.
  - $Basis\ Step:P(n):$ ***We can form $n$ cents of postages using just 3-cent stamps and 10-cent stamps. Form the tabel above, $P(18)$ is true.***
  - $Inductive\ Step:$ ***Assume that we can form $k$ cents of postage, Then if it included two 10-cent stamps, replace them by seven 3-cent stamps. Otherwise, it is formed either from just 3-cent stamps or from one 10-cemt stamp and $k-10$ cents in 3-cent stamps. Replace three 3-cent stamps by one 10-cent stamp ,and then we can get $k+1$ cents in postage.***
- (c) Prove your answer to (a) using strong induction. How does the inductive hypothesis in this proof differ from that in the inductive hypothesis for a proof using mathematical induction?
  - ***Assume that $\forall{j\in[18,k]}P(j)$, where $k$ is an integer greater than or equal to $20$. To show that $P(k+1)$ is true, we already knew that $P(k-2)$ is true because $k\geq{18}$, then we just simply add another 3-cent stamp to it, thus $k+1$ cents postage will be formed.***

**12 . Use strong induction to show that every positive integer $n$ can be written as a sum of distinct powers of two, that is, as a sum of a subset of the integers $2^0 =1,2^1 =2,2^2 =4$, and so on. [Hint: For the inductive step, separately consider the case where $k + 1$ is even and where it is odd. When it is even, note that $(k + 1)/2$ is an integer.]**
- ***Assume that $P(k)$ holds, that is, every integer up to $k$ can be written as a sum of distinct powers of two, we want to know if $P(k+1)$ holds.***  
  ***If $k+1$ is odd, then we can just add $2^0=1$ to it.***
  ***If $k+1$ is even, then $\frac{(k+1)}{2}$ is an positive integer. By the inductive hypothesis, we know that $P(\frac{(k+1)}{2})$ holds.***
  $\frac{(k+1)}{2}=2^a+2^b+2^c+..., (\forall{a,b,c,...}\in{\mathbb{N}})$
  $(k+1)=2\times(2^a+2^b+2^c+...)=2^{a+1}+2^{b+1}+2^{c+1}+..., (\forall{a,b,c,...}\in{\mathbb{N}})$
  ***As shown, $P(k+1)$ holds if $P(k)$ holds.***
  

**26 . Suppose that $P (n)$ is a propositional function. Determine for which nonnegative integers $n$ the statement $P (n)$ must be true if**
- (b) $P(0)$ is true; for all nonnegetive integers $n$, if $P(n)$is true then $P(n+3)$ is true.
  - $n:\{x|x=3n, \forall{n\in{\mathbb{N}}}\}$

- (d) $P(0)$ is true; for all nonnegative integers $n$, if $P (n)$ is true, then $P(n + 2)$ and $P(n + 3)$ are true.
  - $n:\{x|x\in{\mathbb{N}}\land x\neq{1}\}$

**32 . Find  the  flaw  with  the  following  “proof”  that  every postage of three cents or more can be formed using just $3$-cent and $4$-cent stamps.  
$Basis\ Step:$ We can form postage of three cents with a single $3$-cent stamp and we can form postage of four cents using a single $4$-cent stamp.  
$Inductive\ Step:$ Assume that we can form postage of $j$ cents for all nonnegative integers $j$ with $j\leq k$ using just $3$-cent and $4$-cent stamps. We can then form postage of $k + 1$ cents by replacing one $3$-cent stamp with a $4$-cent stamp or by replacing two $4$-cent stamps by three $3$-cent stamps.**
1. ***$j$ shuold be greater than or equal to $3$.***
2. ***It doesn't hold at $j=5$.***

## Section 5-3

**8 . Give a recursive definition of the sequence $\{a_n\}$, $n = 1,2,3,...$ if**
- (a) $a_n =4n-2$.
  - $a_n=a_{n-1}+4, a_1=2, \forall{n}\in{\mathbb{N}}\geq{2}$
- (c) $a_n =n(n+1)$.
  - $a_n=a_{n-1}+2n, a_1=2, \forall{n}\in{\mathbb{N}}\geq{2}$

**12 . Prove that $f_1^2 +f_2^2 +...+f_n^2 = f_nf_{n+1}$ when $n$ is a positive integer. ($f_n$ is the $n$ th Fibonacci number.)**
- $Basis\ Step: n=1, f_1^2=f_1f_2=1^2.$
- $Inductive\ Step:$ ***Assume that when*** $n=k, \sum\limits_{i=1}^{k}f_i^2=f_kf_{k+1}$
  ***Then when*** $n=k+1, \sum\limits_{i=1}^{k+1}f_i^2=\sum\limits_{i=1}^{k}f_i^2+f_{k+1}^2=f_kf_{k+1}+f_{k+1}^2=f_{k+1}(f_k+f_{k+1})=f_{k+1}f_{k+2}$. 
  ***So $\sum\limits_{i=1}^{n}f_n^2=f_nf_{n+1}$. By mathematical induction.***

**26 . Let $S$ be the subset of the set of ordered pairs of integers defined recursively by Basis step: $(0, 0) \in S$. Recursive step: If $(a,b) \in S$, then $(a + 2,b + 3) \in S$ and $(a+3,b+2)\in S$.**
- (a) List the elements of $S$ produced by the first five applications of the recursive definition.
  - $S:\{(0,0),(2,3),(3,2),(4,6),(5,5),(6,4),(6,9),(7,8),(8,7),(9,6),(8,12),(9,11)$
    $(10,10),(11,9),(12,8),(10,15),(11,14),(12,13),(13,12),(14,11),(15,10)\}$
- (b) Use strong induction on the number of applications of the recursive ste of  the definition to show that $5|a+b$ when $(a,b)\in S$.
  - ***Let $P(n):5|a+b,$ whenever ${(a,b)}\in S$ is obtained by n applications of the recursive step.***
  - ***$Basis\ Step: n=0, P(0)$ is true because $5|0+0$***
    ***$Inductive\ Step:$ Assume the strong inductive hypothesis that for every fixed $k,P(j),\ \forall{j}(0\leq{j}\leq{k})$***
    ***Then when*** $n=k+1,\ 5|a+2+b+3$ ***Since $5|a+b$ and $5|2+3$.***
- (c) Use structural induction to show that $5 | a + b$ when $(a,b)\in S$.
  - ***Same as (b), it holds for P(0).***
</font>